theories/Math/SetTheory.v
@@ -375,10 +375,6 @@ Definition _Card_mul : Card -> Card -> Card :=
 Definition _Card_exp : Card -> Card -> Card :=
   Cardinality.exp.
 
-Section HARTOGS.
-
-End HARTOGS.
-
 Definition cutoff (D : Type@{Set_u}) : Tree :=
   mkNode (B.sig (D -> D -> Prop) (@well_founded D)) (fun RWF => @fromWfSet D RWF.(B.proj1_sig) RWF.(B.proj2_sig)).
 
